...일단 커밋

src/lean/Nemonuri/Study/StanfordOnline/Compilers/Introduction/Program.lean
@@ -7,17 +7,19 @@ public section public_s
 
 namespace Nemonuri.Study.StanfordOnline.Compilers
 
-universe u
+universe u u1 u2
 set_option autoImplicit false
 
 
 namespace Program
 
 
-
 namespace Runtime
 
-namespace State
+structure TypeContext : Type (u+1) where
+  TProgram : Type u
+  TData : Type u
+  TOutput : Type u
 
 inductive Label where
   | load
@@ -25,40 +27,181 @@ inductive Label where
   | produceOutput
   deriving DecidableEq
 
-instance Label.instLawfulBEq : LawfulBEq Label := inferInstance
+
+namespace Label
+
+instance instLawfulBEq : LawfulBEq Label := inferInstance
+
+-- Note: 대체 이건 무슨 패턴이지...?
+-- https://github.com/leanprover/lean4/blob/v4.30.0-rc2/src/Init/Control/State.lean
+
+/-
+protected def ToSort (toSort: Label → Sort u) : Sort u := (label: Label) → toSort label
+
+protected def ToSort.mk {toSort: Label → Sort u} {label: Label} (x: toSort label) := x
+
+protected def OfSort (_: Sort u) : Type := Label
+
+protected def OfSort.mk {_: Sort u} (x: Label) := x
+-/
+
+def Motive : Type u := Label → Sort u
+
+def Motive.mk (self: Label → Sort u) : Motive := self
 
 
-structure TypeContext : Type (u+1) where
-  TProgram : Type u
-  TData : Type u
-  TOutput : Type u
+class Motive.LiftM (TPre: semiOutParam Motive.{u}) (TPost: Motive.{u}) where
+  liftM (label) : TPre label → TPost label
 
 
-end State
+end Label
+
+/-
+class OfLabelM (T: Type u1) (m: Type u1 → Type u2) where
+  ofLabel: Label → m T
+
+class ToLabelM (T: Type u1) (m: Type u1 → Type u2) where
+  toLabel: m T → Label
+
+abbrev OfLabel T := OfLabelM T Id
+
+abbrev ToLabel T := ToLabelM T Id
+-/
+
+/-
+open Label Motive in
+class StepM TPre TPost [inst: LiftM.{u} TPre TPost] where
+  step (label) : (TPre label) → (LiftM.liftM label (TPre label))
+-/
 
 
-inductive State (tc: State.TypeContext) : State.Label → Type u where
+--class LogM (m1 m2: (label: Label) → Sort u) where
+--  log {}
+
+
+inductive State (tc: TypeContext) : Label → Type u where
+  | load : tc.TProgram → State tc .load
+  | takeInput : tc.TData → tc.TProgram → State tc .takeInput
+  | produceOutput : tc.TOutput → tc.TProgram → State tc .produceOutput
+
+def Label.Motive.ofState (tc: TypeContext) : Label.Motive := State tc
+
+--instance State.instStepM {tc} : StepM id (State tc) where
+--  step _ := id
+  --TMotivePost := State tc
+/-
+    match label with
+    | .load => tc.TProgram
+    | .takeInput => tc.TData × tc.TProgram
+    | .produceOutput => tc.TOutput × tc.TProgram
+-/
+  --trace _ := id
+/-
+    match label, pre with
+    | .load, prog => State.load prog
+    | .takeInput, ⟨data, prog⟩ => State.takeInput data prog
+    | .produceOutput, ⟨output, prog⟩ => State.produceOutput output prog
+-/
+
+
+
+inductive Trace (tc: TypeContext) : Label → Type u where
   | load :
-      tc.TProgram →
-      State tc .load
-  | takeInput {label: State.Label} :
-      State tc label →
-      tc.TData →
-      tc.TProgram →
-      State tc .takeInput
-  | produceOutput :
+      State tc .load →
+      Trace tc .load
+  | takeInput :
+      (label: Label) →
+      Trace tc label →
       State tc .takeInput →
-      tc.TOutput →
-      tc.TProgram →
-      State tc .produceOutput
+      Trace tc .takeInput
+  | produceOutput :
+      Trace tc .takeInput →
+      State tc .produceOutput →
+      Trace tc .produceOutput
+
+def Label.Motive.ofTrace (tc: TypeContext) : Label.Motive := Trace tc
+
+instance Trace.instTraceM {tc} : TraceM (Trace tc) where
+  TMotivePre label :=
+    match label with
+    | .load => State tc .load
+    | .takeInput => (label: Label) × (Trace tc label) × (State tc .takeInput)
+    | .produceOutput =>
 
 
+
+--inductive StateM (tc: TypeContext) (m: (label: State.Label) → State tc label → (Type u))
+
+namespace History
+
+protected inductive Raw (tc: TypeContext) : State.Label → Type u where
+  | load :
+      State tc .load →
+      History.Raw tc .load
+  | takeInput :
+      (label: State.Label) →
+      History.Raw tc label →
+      State tc .takeInput →
+      History.Raw tc .takeInput
+  | produceOutput :
+      History.Raw tc .takeInput →
+      State tc .produceOutput →
+      History.Raw tc .produceOutput
+
+end History
+
+structure History (tc: TypeContext) where
+  label: State.Label
+  raw: History.Raw tc label
+
+abbrev History.Raw.toHistory {tc label} (raw: History.Raw tc label) : History tc := .mk label raw
+
+
+namespace History
+
+open Raw
+
+variable {tc: TypeContext}
+
+@[match_pattern]
+def load (prog: tc.TProgram) : History tc :=
+  State.load prog |> Raw.load |> toHistory
+
+@[match_pattern]
+def takeInput (label) (pre: History.Raw tc label) (data: tc.TData) (prog: tc.TProgram) : History tc :=
+  State.takeInput data prog |> Raw.takeInput label pre |> toHistory
+
+@[match_pattern]
+def produceOutput (pre: History.Raw tc .takeInput) (output: tc.TOutput) (prog: tc.TProgram) : History tc :=
+  State.produceOutput output prog |> Raw.produceOutput pre |> toHistory
+
+@[simp, spec]
+theorem load_label_eq (prog: tc.TProgram) : (load prog).label = .load := by
+  unfold load
+  simp
+
+@[simp, spec]
+theorem takeInput_label_eq label pre (data: tc.TData) (prog: tc.TProgram)
+  : (takeInput label pre data prog).label = .takeInput := by
+  unfold takeInput
+  simp
+
+@[simp, spec]
+theorem produceOutput_label_eq pre (output: tc.TOutput) (prog: tc.TProgram)
+  : (produceOutput pre output prog).label = .produceOutput := by
+  unfold produceOutput
+  simp
+
+end History
+
+
+/-
 def toProgram {tc label} (state: State tc label) : tc.TProgram :=
   match state with
   | .load prog => prog
   | .takeInput _ _ prog => prog
   | .produceOutput _ _ prog => prog
-
+-/
 
 namespace State
 
@@ -76,6 +219,56 @@ end State
 
 open State
 
+namespace Step
+
+class Load (tc: TypeContext) where
+  load: tc.TProgram → State tc .load
+
+class TakeInput (tc: TypeContext) (req: Label.Req) where
+  takeInput (label: Label) : (req label) → (State tc label) → (State tc .takeInput)
+
+class ProduceOutput (tc: TypeContext) where
+  produceOutput :
+    State tc .takeInput →
+    State tc .produceOutput
+
+end Step
+
+
+protected class abbrev Raw (tc: TypeContext) (req: Label.Req) :=
+  Step.Load tc, Step.TakeInput tc req, Step.ProduceOutput tc
+
+end Runtime
+
+open Runtime State in
+class Runtime (tc: TypeContext) where
+  req: Label.Req
+  raw: Runtime.Raw tc req
+
+namespace Runtime
+
+
+abbrev Raw.toRuntime {tc req} (self: Runtime.Raw tc req) : Runtime tc := Runtime.mk req self
+
+abbrev Step.Spec tc := Step tc → Prop
+
+abbrev PlausibleState {tc} (spec: Step.Spec tc) := Subtype spec
+
+
+namespace PlausibleStep
+
+variable {tc: TypeContext} {spec: Step.Spec tc}
+
+def load
+
+
+
+end PlausibleStep
+
+
+
+
+
 class HasState (tc: TypeContext) (T: Type u)
   extends HasSnapShot tc T where
   setState (before: T) (arg: SnapShot tc) : T--{ after: T // (snapShot after) = arg }
@@ -90,6 +283,7 @@ class Init (tc: TypeContext) where
   init_spec {label: Label} (pre: State tc label) : ∀prog, match init pre prog with | .init prog2 => prog = prog2
 -/
 
+/-
 class TakeInput (tc: TypeContext) where
   takeInput_req {label: Label} (state: State tc label) : Prop
   takeInput {label: Label} :
@@ -99,14 +293,17 @@ class TakeInput (tc: TypeContext) where
   takeInput_spec {label} (pre: Subtype (@takeInput_req label)) data :
     match takeInput pre data with
     | .takeInput pre2 data2 _ => pre ≍ pre2 ∧ data = data2
+-/
 
-abbrev TakeInput.ReqState {tc} (self: TakeInput tc) label := Subtype (@self.takeInput_req label)
+--abbrev TakeInput.ReqState {tc} (self: TakeInput tc) label := Subtype (@self.takeInput_req label)
 
+/-
 class ProduceOutput (tc: TypeContext) where
   produceOutput :
     State tc .takeInput →
     State tc .produceOutput
   produceOutput_spec : ∀pre, match produceOutput pre with | .produceOutput pre2 _ _ => pre = pre2
+-/
 
 end Runtime
 
